% Copyright 2024 Kieran W Harvie. All rights reserved.

\section{Bernstein Basis Polynomials}
The $k^\text{th}$ Bernstein basis polynomial of order $n$ is defined as:
\[
	b_{k,n}(t) = \binom{n}{k}(1-t)^{n-k}t^k
\]
Where we follow that convention that $\binom{n}{k}=0$ when $k<0$ or $k>n$.
\\

They have some really useful properties that lend them themselves to applications like
approximating continuous functions,
numerically stable polynomial evaluation, 
and are the foundation of BÃ©zier geometry.
To this end it will be useful to collect some of those properties bellow.
\begin{center}
\begin{tikzpicture}[domain=0:1,scale=5]
	\draw[red] plot (\x,{(1-\x)^3});
	\draw[blue] plot(\x,{3*\x*(1-\x)^2});
	\draw[yellow] plot (\x,{3*\x*\x*(1-\x)});
	\draw[green] plot (\x,{\x*\x*\x});

	\draw[<->] (0,1.1)--(0,0)--(1.1,0);
\end{tikzpicture}

The four Bernstein basis polynomials of degree three over $[0,1]$.
\end{center}

\subsubsection{Fundamental Recursion:}
The most fundamental property of Bernstein basis polynomials is the recursion:
\[b_{k,n+1}(t) = (1-t)b_{k,n}(t)+tb_{k-1,n}(t)\]
And that there are $n+1$ polynomials of order $n$,
since when $k<0$ or $k>n$ we have:
\[b_{k,n}(t) = 0\]
Both of these properties can be verified by inspection of the definition and let us create a table of low order Bernstein basis polynomials to further cultivate intuition:
\[
\begin{array}{|c|ccccc|}
	\hline
	b_{k,n}(t)&0&1&2&3&4\\
	\hline
	4&(1-t)^4&4t(1-t)^3&6t^2(1-t)^2&4t^3(1-t)&t^4\\
	3&(1-t)^3&3t(1-t)^2&3t^2(1-t)&t^3&\\
	2&(1-t)^2&2t(1-t)&t^2&&\\
	1&1-t&t&&&\\
	0&1&&&&\\
	\hline
\end{array}
\]

\subsubsection{Endpoints:}
In most application we will be considering $t\in[0,1]$.
So it makes sense to consider $b_{k,n}(0)$ and $b_{k,n}(1)$ as the `endpoints' and note  their values as:
\[b_{k,n}(0) = \begin{cases}1& k=0\\0&k\neq0\\\end{cases}\quad\text{and}\quad b_{k,n}(1) = \begin{cases}1& k= n\\0&k\neq n\\\end{cases}\]

\subsubsection{Product:}
The product of two Bernstein basis polynomials is another one:
\[\begin{aligned}
	b_{k,n}(t)b_{l,m}(t) =& \binom{n+m}{k+l}^{-1}\binom{n}{k}\binom{m}{l}b_{k+l,n+m}(t)\\
	=&\binom{n+m}{m}^{-1}\binom{k+l}{l}\binom{n+m-(k+l)}{m-l}b_{k+l,n+m}(t)\\
\end{aligned}\]

\subsubsection{Inner Product and Partition of Unity:}
The following combinatorial identity can be verified by expansion:
\[\binom{n}{l}\binom{l}{k} = \binom{n}{k}\binom{n-k}{l-k}\]
When combined with the binomial theorem it allows us evaluate an `inner product' of Bernstein basis polynomials:
\[\begin{aligned}
	\sum_{l=k}^nb_{k,l}(t)b_{l,n}(\tau) =& \sum_{l=k}^n\binom{n}{l}\binom{l}{k}t^l\tau^k(1-t)^{n-l}(1-\tau)^{l-k}\\
	=& \binom{n}{k}(t\tau)^k\sum_{l=k}^n\binom{n-k}{l-k}(1-t)^{n-l}(t(1-\tau))^{l-k}\\
	=& \binom{n}{k}(t\tau)^k\sum_{l=0}^{n-k}\binom{n-k}{l}(1-t)^{n-l-k}(t(1-\tau))^{l}\\
	=& \binom{n}{k}(t\tau)^k(1-t+t(1-\tau))^{n-k}\\
	=& b_{k,n}(t\tau)\\
\end{aligned}\]
In particular,
when $k$ and $\tau$ equal $0$, we have:
\[b_{k,l}(\tau) = b_{k,n}(t\tau) = 1\]
Which substitution into the general case gives:
\[\sum_{l=0}^nb_{l,n}(t) = 1\]
Hence,
for any given $n$,
the polynomials $b_{k,n}(t)$ are a partition of unity.

\subsubsection{Reflection:}
From the following binomial formula:
\[\binom{n}{k}=\binom{n}{n-k}\]
We get the following formula for reflecting argument around $\frac{1}{2}$:
\[b_{k,n}(t) = b_{n-k,n}(1-t)\]
Which gives my favourite Bernstein basis polynomial formula: 
\[ b_{k,m}(\tau+(1-\tau)t) = \sum_{l=0}^kb_{k-l,n-l}(\tau)b_{l,n}(t) \]
By applying the reflection to the inner product formula:
\[\begin{aligned}
	b_{k,n}(\tau+(1-\tau)t) =& b_{k,n}(1-(1-t)(1-\tau))\\
	=& b_{n-k,n}((1-t)(1-\tau))\\
	=&\sum_{l=n-k}^nb_{n-k,l}(1-\tau)b_{l,n}(1-t)\\
	=&\sum_{l=n-k}^nb_{k-(n-l),l}(\tau)b_{n-l,n}(t)\\
\end{aligned}\]
And then change the summation order so $l$ goes down from $n$ instead of up from $n-k$.

\subsubsection{Bounds:}
When $t\in[0,1]$ we have both $t\geq0$ and $1-t\geq0$ and hence:
\[t\in [0,1] \Rightarrow b_{k,n}(t)\geq0 \]
Now since each individual polynomial is positive we have:
\[b_{k,n}(t) \leq \sum_{k=0}^nb_{k,n}(t) = 1\]

\subsubsection{Derivative:}
By direct application of the product rule we get:
\[b_{k,n+1}'(t) = k\binom{n+1}{k}(1-t)^{n+1-k}t^{k-1}-(n+1-k)\binom{n+1}{k}(1-t)^{n-k}t^k\]
Simpling the coefficients containing $k$ into the binomial coefficients we obtain:
\[b_{k,n+1}'(t) = (n+1)(b_{k-1,n}(t)-b_{k,n}(t))\]
If we instead factor common terms we get:
\[b_{k,n+1}'(t) = (1-t)^{n-k}t^{k-1}\binom{n+1}{k}\bigg(k(1-t)-(n+1-k)t\bigg)\]
When $t\in(0,1)$ the first three factors are non-negative,
hence there can only be an extrema where the fourth factor is zero at $t=\frac{k}{n+1}$.
By considering the endpoints this extrema must be a maximum and is the only extrema on $t\in[0,1]$.

\subsubsection{Useful Sums:}
We have already used binomial expansion when calculating the inner product.
However, if we consider the general expression:
\[(x+y)^n = \sum_{k=0}^n\binom{n}{k}x^{n-k}y^k\]	
When derived by $y$:
\[n(x+y)^{n-1} = \sum_{k=0}^nk\binom{n}{k}x^{n-k}y^{k-1}\]
Multiplied by $y(x+y)$:
\[ny(x+y)^n = (x+y)\sum_{k=0}^nk\binom{n}{k}x^{n-k}y^k\]
And having set $x=1-t$ and $y=t$:
\[nt = \sum_{k=0}^nk\binom{n}{k}(1-t)^{n-k}t^k\ = \sum_{k=0}^nkb_{k,n}(t)\]
We get this sum with simple terms.
The simplicity makes it a useful starting point and sanity check when writing algorithms involving the Bernstein basis polynomials.
For example,
if we are writing an algorithm for calculating the value of a Bernstein basis expansion at $t$ we know that if we choose linearly increasing coefficients we should get a linear function of $t$.
If we conversely want the Bernstein basis expansion of a linear function we know to use linearly increasing coefficients.	
\\

Through similar methods we get similar sums for higher powers, for example:
\[n(n-1)t^2 = \sum_{k=0}^nk(k-1)b_{k,n}(t)\]
They are useful for similar starting points and sanity checks for derivatives.
For example if we choose quadratically increasing coefficients in a Bernstein basis expansion we should get a linear derivative.
