% Copyright 2023 Kieran W Harvie. All rights reserved.

\section{Cool Chebyshev Generating Functions}

\subsection{Elementary Generating Functions}

\begin{equation*}
\begin{aligned}
	\sum_{i=0}^{\infty}T_n(x)t^n =& \frac{1-xt}{1-2xt+t^2} \\
	\sum_{i=0}^{\infty}U_n(x)t^n =& \frac{1}{1-2xt+t^2} \\
	\text{With}&\\
	T_n(\cos(\theta)) =& \cos(n\theta)\\
	U_n(\cos(\theta))\sin(\theta) =& \sin((n+1)\theta)\\
\end{aligned}
\end{equation*}
For example:
\begin{equation*}
\begin{aligned}
	\sum_{n=0}^\infty t^n\sum_{k=0}^nT_k(\cos(\theta))
	=& \frac{1}{1-t}\cdot\frac{1-\cos(\theta)t}{1-2\cos(\theta)t+t^2} \\	
	=& \frac{1-t\cos(\theta)}{\sin(\theta)(1-t)}\cdot\frac{\sin(\theta)}{1-2\cos(\theta)t+t^2} \\	
	=& \frac{1-t\cos(\theta)}{\sin(\theta)(1-t)}\sum_{n=0}^{\infty}t^n\sin((n+1)\theta) \\
\end{aligned}
\end{equation*}

\subsection{Complex Exponential}
There's some stuff you can do with the complex exponential.
\\
First is an explanation for the generating function forms:
\begin{equation*}
\begin{aligned}
	\sum_{n=0}^\infty t^n\exp(in\phi) 
	=&\frac{1}{1-t\exp(i\phi)} \\
	=&\frac{1-t\exp(-i\phi)}{1+t^2-2t\cos(\phi)} \\
	=&\frac{1-t(\cos(\phi)-i\sin(\phi))}{1+t^2-2t\cos(\phi)} \\
	=&\sum_{n=0}^\infty t^n\cos(n\phi)+i\sum_{n=0}^\infty t^{n+1}\sin((n+1)\phi)\\ 
\end{aligned}
\end{equation*}
But also stuff like:
\begin{equation*}
\begin{aligned}
	\sum_{n=0}^{\infty}nt^n\exp(in\phi) 
	=& \frac{t\exp(i\phi)}{(1-t\exp(i\phi))^2}\\
	=& \frac{t\exp(i\phi)(1-t\exp(-i\phi))^2}{(1+t^2-2t\cos(\phi))^2} \\
	=& \frac{t\cos(\phi)(1-2t\cos(\phi)+t^2)+t\sin(\phi)(1-2t\sin(\phi)-t^2)}{(1+t^2-2t\cos(\phi))^2} \\
\end{aligned}
\end{equation*}
The notes kind of end here and I don't remember what I was cooking.
The denominator and the $t\cos(\phi)$ factor resemble the generating function but need more massaging.

\subsection{Orthogonality}

Let:
\[f(x,t) = \frac{1-t^2}{1-2tx+t^2} \]
We have:
\[\int_{-1}^1T_n(x)f(x,t)\frac{dx}{\sqrt{1-x^2}}\ = \pi t^n \]

Let $P$ be some polynomial:
\[ P(x) = \sum_{n}p_nT_n(x) \]
Then:
\[ P(x) = (1-2tx+t^2)Q(x,t)+P\left(\frac{1+t^2}{2t}\right) \]
For some polynomial $Q$ with coefficients dependent on $t$.
\\
Let $q(t)$ be the coefficient from polynomial $T_0(x)$.
\\
Then:
\[\pi\sum_np_nt^n = \int_{-1}^1P(x)f(x,t)\frac{dx}{\sqrt{1-x^2}} = \pi q(t)(1-t^2) + P\left(\frac{1+t^2}{2t}\right) \]

Derive and sub $t=\pm1$ to get:
\[\sum_nnp_n = -2q(1)\]
\[\sum_nnp_n(-1)^n = 2q(-1)\]

Might work for some general function, not sure.
